<?xml version="1.0"?>
<rdf:RDF xmlns="http://purl.org/nampi/owl/core#"
     xml:base="http://purl.org/nampi/owl/core"
     xmlns:owl="http://www.w3.org/2002/07/owl#"
     xmlns:rdf="http://www.w3.org/1999/02/22-rdf-syntax-ns#"
     xmlns:xml="http://www.w3.org/XML/1998/namespace"
     xmlns:xsd="http://www.w3.org/2001/XMLSchema#"
     xmlns:rdfs="http://www.w3.org/2000/01/rdf-schema#"
     xmlns:skos="http://www.w3.org/2004/02/skos/core#">
    <owl:Ontology rdf:about="http://purl.org/nampi/owl/core">
        <owl:versionIRI rdf:resource="http://purl.org/nampi/owl/core/0.2.1"/>
        <owl:imports rdf:resource="http://erlangen-crm.org/211015/"/>
    </owl:Ontology>
    


    <!-- 
    ///////////////////////////////////////////////////////////////////////////////////////
    //
    // Object Properties
    //
    ///////////////////////////////////////////////////////////////////////////////////////
     -->

    


    <!-- http://purl.org/nampi/owl/core#adds_aspect -->

    <owl:ObjectProperty rdf:about="http://purl.org/nampi/owl/core#adds_aspect">
        <rdfs:subPropertyOf rdf:resource="http://purl.org/nampi/owl/core#uses_aspect"/>
        <owl:inverseOf rdf:resource="http://purl.org/nampi/owl/core#aspect_is_added_in"/>
        <rdfs:comment xml:lang="en">A new aspect is related to the main person of the event. This can mean, for instance, that a new status is acquired or a new occupation is started.</rdfs:comment>
        <rdfs:label xml:lang="en">adds aspect</rdfs:label>
    </owl:ObjectProperty>
    


    <!-- http://purl.org/nampi/owl/core#aspect_is_added_in -->

    <owl:ObjectProperty rdf:about="http://purl.org/nampi/owl/core#aspect_is_added_in">
        <rdfs:subPropertyOf rdf:resource="http://purl.org/nampi/owl/core#aspect_is_used_in"/>
        <rdfs:comment xml:lang="en">A new aspect is related to the main person of the event. This can mean, for instance, that a new status is acquired or a new occupation is started.</rdfs:comment>
        <rdfs:label xml:lang="en">aspect is added in</rdfs:label>
    </owl:ObjectProperty>
    


    <!-- http://purl.org/nampi/owl/core#aspect_is_removed_in -->

    <owl:ObjectProperty rdf:about="http://purl.org/nampi/owl/core#aspect_is_removed_in">
        <rdfs:subPropertyOf rdf:resource="http://purl.org/nampi/owl/core#aspect_is_used_in"/>
        <owl:inverseOf rdf:resource="http://purl.org/nampi/owl/core#removes_aspect"/>
        <rdfs:comment xml:lang="en">A pre-existing relationship between the main participant of the event and the aspect is severed. This can mean, for instance, that a status is lost or an occupation is stopped.</rdfs:comment>
        <rdfs:label xml:lang="en">aspect is removed in</rdfs:label>
    </owl:ObjectProperty>
    


    <!-- http://purl.org/nampi/owl/core#aspect_is_used_in -->

    <owl:ObjectProperty rdf:about="http://purl.org/nampi/owl/core#aspect_is_used_in">
        <rdfs:subPropertyOf rdf:resource="http://erlangen-crm.org/211015/P67i_is_referred_to_by"/>
        <rdfs:subPropertyOf rdf:resource="http://www.w3.org/2002/07/owl#topObjectProperty"/>
        <owl:inverseOf rdf:resource="http://purl.org/nampi/owl/core#uses_aspect"/>
        <rdfs:comment xml:lang="en">Connects an aspect to an event it is relevant to / was used in. Being connected to an event means this aspect is related to the main participant of the event and in a lesser degree to the other participants.</rdfs:comment>
        <rdfs:label xml:lang="en">aspect is used in</rdfs:label>
    </owl:ObjectProperty>
    


    <!-- http://purl.org/nampi/owl/core#authors -->

    <owl:ObjectProperty rdf:about="http://purl.org/nampi/owl/core#authors">
        <rdfs:subPropertyOf rdf:resource="http://erlangen-crm.org/211015/P14i_performed"/>
        <rdfs:subPropertyOf rdf:resource="http://www.w3.org/2002/07/owl#topObjectProperty"/>
        <owl:inverseOf rdf:resource="http://purl.org/nampi/owl/core#is_authored_by"/>
        <rdfs:comment xml:lang="en">Connects an author to a document interpretation act which means that the author is responsible for the interpretation.</rdfs:comment>
        <rdfs:label xml:lang="en">authors</rdfs:label>
    </owl:ObjectProperty>
    


    <!-- http://purl.org/nampi/owl/core#changes_aspect_related_to -->

    <owl:ObjectProperty rdf:about="http://purl.org/nampi/owl/core#changes_aspect_related_to">
        <rdfs:subPropertyOf rdf:resource="http://purl.org/nampi/owl/core#has_other_participant"/>
        <owl:inverseOf rdf:resource="http://purl.org/nampi/owl/core#is_related_to_changed_aspect_in"/>
        <rdfs:comment xml:lang="en">Signifies that aspects related to the event are also related to the secondary actor. In case of a group, this can mean for instance that a status was valid inside the group or that an occupation had the actor as employer.</rdfs:comment>
        <rdfs:label xml:lang="en">changes aspect related to</rdfs:label>
    </owl:ObjectProperty>
    


    <!-- http://purl.org/nampi/owl/core#contains_source_location -->

    <owl:ObjectProperty rdf:about="http://purl.org/nampi/owl/core#contains_source_location">
        <rdfs:subPropertyOf rdf:resource="http://erlangen-crm.org/211015/P165_incorporates"/>
        <rdfs:subPropertyOf rdf:resource="http://www.w3.org/2002/07/owl#topObjectProperty"/>
        <owl:inverseOf rdf:resource="http://purl.org/nampi/owl/core#has_source"/>
        <rdfs:comment xml:lang="en">A source contains a source location, for example, a book contains a specific page as specified by a particular page number or a website contains a specific individual web page.</rdfs:comment>
        <rdfs:label xml:lang="en">contains source location</rdfs:label>
    </owl:ObjectProperty>
    


    <!-- http://purl.org/nampi/owl/core#dies_in -->

    <owl:ObjectProperty rdf:about="http://purl.org/nampi/owl/core#dies_in">
        <rdfs:subPropertyOf rdf:resource="http://purl.org/nampi/owl/core#is_main_participant_in"/>
        <owl:inverseOf rdf:resource="http://purl.org/nampi/owl/core#ends_life_of"/>
        <rdfs:comment xml:lang="en">Specifies that the event is about the end of the life of the main participant.</rdfs:comment>
        <rdfs:label xml:lang="en">dies in</rdfs:label>
    </owl:ObjectProperty>
    


    <!-- http://purl.org/nampi/owl/core#ends_life_of -->

    <owl:ObjectProperty rdf:about="http://purl.org/nampi/owl/core#ends_life_of">
        <rdfs:subPropertyOf rdf:resource="http://purl.org/nampi/owl/core#has_main_participant"/>
        <rdfs:range rdf:resource="http://purl.org/nampi/owl/core#person"/>
        <rdfs:comment xml:lang="en">Specifies that the event is about the end of the life of the main participant.</rdfs:comment>
        <rdfs:label xml:lang="en">ends life of</rdfs:label>
    </owl:ObjectProperty>
    


    <!-- http://purl.org/nampi/owl/core#has_date -->

    <owl:ObjectProperty rdf:about="http://purl.org/nampi/owl/core#has_date">
        <rdfs:subPropertyOf rdf:resource="http://erlangen-crm.org/211015/P129_is_about"/>
        <rdfs:subPropertyOf rdf:resource="http://www.w3.org/2002/07/owl#topObjectProperty"/>
        <rdfs:domain rdf:resource="http://purl.org/nampi/owl/core#event"/>
        <rdfs:range rdf:resource="http://purl.org/nampi/owl/core#date"/>
        <rdfs:comment xml:lang="en">Connects an event with a date it is related to / describes.</rdfs:comment>
        <rdfs:label xml:lang="en">has date</rdfs:label>
    </owl:ObjectProperty>
    


    <!-- http://purl.org/nampi/owl/core#has_interpretation -->

    <owl:ObjectProperty rdf:about="http://purl.org/nampi/owl/core#has_interpretation">
        <rdfs:subPropertyOf rdf:resource="http://erlangen-crm.org/211015/P140_assigned_attribute_to"/>
        <rdfs:subPropertyOf rdf:resource="http://www.w3.org/2002/07/owl#topObjectProperty"/>
        <owl:inverseOf rdf:resource="http://purl.org/nampi/owl/core#is_interpretation_of"/>
        <rdfs:domain rdf:resource="http://purl.org/nampi/owl/core#act"/>
        <rdfs:range rdf:resource="http://purl.org/nampi/owl/core#event"/>
        <rdfs:comment xml:lang="en">Connects a event to a document interpretation act.</rdfs:comment>
        <rdfs:label xml:lang="en">has interpretation</rdfs:label>
    </owl:ObjectProperty>
    


    <!-- http://purl.org/nampi/owl/core#has_main_participant -->

    <owl:ObjectProperty rdf:about="http://purl.org/nampi/owl/core#has_main_participant">
        <rdfs:subPropertyOf rdf:resource="http://purl.org/nampi/owl/core#has_participant"/>
        <owl:inverseOf rdf:resource="http://purl.org/nampi/owl/core#is_main_participant_in"/>
        <rdfs:range rdf:resource="http://purl.org/nampi/owl/core#person"/>
        <rdfs:comment xml:lang="en">Declares a person to be the main participant of a specific event.</rdfs:comment>
        <rdfs:label xml:lang="en">has main participant</rdfs:label>
    </owl:ObjectProperty>
    


    <!-- http://purl.org/nampi/owl/core#has_other_participant -->

    <owl:ObjectProperty rdf:about="http://purl.org/nampi/owl/core#has_other_participant">
        <rdfs:subPropertyOf rdf:resource="http://purl.org/nampi/owl/core#has_participant"/>
        <owl:inverseOf rdf:resource="http://purl.org/nampi/owl/core#is_other_participant_in"/>
        <rdfs:comment xml:lang="en">Signifies that an actor is a secondary participant in the real-life event depicted by the event.</rdfs:comment>
        <rdfs:label xml:lang="en">has other participant</rdfs:label>
    </owl:ObjectProperty>
    


    <!-- http://purl.org/nampi/owl/core#has_parent -->

    <owl:ObjectProperty rdf:about="http://purl.org/nampi/owl/core#has_parent">
        <rdfs:subPropertyOf rdf:resource="http://purl.org/nampi/owl/core#has_other_participant"/>
        <owl:inverseOf rdf:resource="http://purl.org/nampi/owl/core#is_parent_in"/>
        <rdfs:comment xml:lang="en">Signifies that the actor functions starts being counted as parent of the main person in the event.</rdfs:comment>
        <rdfs:label xml:lang="en">has parent</rdfs:label>
    </owl:ObjectProperty>
    


    <!-- http://purl.org/nampi/owl/core#has_part -->

    <owl:ObjectProperty rdf:about="http://purl.org/nampi/owl/core#has_part">
        <rdfs:subPropertyOf rdf:resource="http://erlangen-crm.org/211015/P107_has_current_or_former_member"/>
        <rdfs:subPropertyOf rdf:resource="http://www.w3.org/2002/07/owl#topObjectProperty"/>
        <owl:inverseOf rdf:resource="http://purl.org/nampi/owl/core#is_part_of"/>
        <rdfs:comment xml:lang="en">Specifies that an actor is or was a member of a specific group.</rdfs:comment>
        <rdfs:label xml:lang="en">has part</rdfs:label>
    </owl:ObjectProperty>
    


    <!-- http://purl.org/nampi/owl/core#has_participant -->

    <owl:ObjectProperty rdf:about="http://purl.org/nampi/owl/core#has_participant">
        <rdfs:subPropertyOf rdf:resource="http://erlangen-crm.org/211015/P129_is_about"/>
        <rdfs:subPropertyOf rdf:resource="http://www.w3.org/2002/07/owl#topObjectProperty"/>
        <owl:inverseOf rdf:resource="http://purl.org/nampi/owl/core#participates_in"/>
        <rdfs:domain rdf:resource="http://purl.org/nampi/owl/core#event"/>
        <rdfs:range rdf:resource="http://purl.org/nampi/owl/core#actor"/>
        <rdfs:comment xml:lang="en">Connects an actor to a event. It means that the actor is in one way or another involved in the real-life event the event depicts.</rdfs:comment>
        <rdfs:label xml:lang="en">has participant</rdfs:label>
    </owl:ObjectProperty>
    


    <!-- http://purl.org/nampi/owl/core#has_sorting_date -->

    <owl:ObjectProperty rdf:about="http://purl.org/nampi/owl/core#has_sorting_date">
        <rdfs:subPropertyOf rdf:resource="http://purl.org/nampi/owl/core#has_date"/>
        <rdfs:comment xml:lang="en">A date that can be used to sort lists of dates. Doesn&apos;t neccessarily mean the real-life event happened on exactly this date, only that when present in a list of other events sorted by date, the sorting date should be used to determine the exact position in the list.</rdfs:comment>
        <rdfs:label xml:lang="en">has sorting date</rdfs:label>
    </owl:ObjectProperty>
    


    <!-- http://purl.org/nampi/owl/core#has_source -->

    <owl:ObjectProperty rdf:about="http://purl.org/nampi/owl/core#has_source">
        <rdfs:subPropertyOf rdf:resource="http://erlangen-crm.org/211015/P165i_is_incorporated_in"/>
        <rdfs:subPropertyOf rdf:resource="http://www.w3.org/2002/07/owl#topObjectProperty"/>
        <rdfs:domain rdf:resource="http://purl.org/nampi/owl/core#source_location"/>
        <rdfs:range rdf:resource="http://purl.org/nampi/owl/core#source"/>
        <rdfs:comment xml:lang="en">Connects a source location to the source it is contained within.</rdfs:comment>
        <rdfs:label xml:lang="en">has source</rdfs:label>
    </owl:ObjectProperty>
    


    <!-- http://purl.org/nampi/owl/core#has_source_location -->

    <owl:ObjectProperty rdf:about="http://purl.org/nampi/owl/core#has_source_location">
        <rdfs:subPropertyOf rdf:resource="http://erlangen-crm.org/211015/P16_used_specific_object"/>
        <rdfs:subPropertyOf rdf:resource="http://www.w3.org/2002/07/owl#topObjectProperty"/>
        <owl:inverseOf rdf:resource="http://purl.org/nampi/owl/core#is_source_location_for"/>
        <rdfs:domain rdf:resource="http://purl.org/nampi/owl/core#act"/>
        <rdfs:range rdf:resource="http://purl.org/nampi/owl/core#source_location"/>
        <rdfs:comment xml:lang="en">Declares the source location a document interpretation act is based on.</rdfs:comment>
        <rdfs:label xml:lang="en">has source location</rdfs:label>
    </owl:ObjectProperty>
    


    <!-- http://purl.org/nampi/owl/core#is_authored_by -->

    <owl:ObjectProperty rdf:about="http://purl.org/nampi/owl/core#is_authored_by">
        <rdfs:subPropertyOf rdf:resource="http://erlangen-crm.org/211015/P14_carried_out_by"/>
        <rdfs:subPropertyOf rdf:resource="http://www.w3.org/2002/07/owl#topObjectProperty"/>
        <rdfs:domain rdf:resource="http://purl.org/nampi/owl/core#act"/>
        <rdfs:range rdf:resource="http://purl.org/nampi/owl/core#author"/>
        <rdfs:comment xml:lang="en">Specifies the author of a document interpretation act.</rdfs:comment>
        <rdfs:label xml:lang="en">is authored by</rdfs:label>
    </owl:ObjectProperty>
    


    <!-- http://purl.org/nampi/owl/core#is_authored_on -->

    <owl:ObjectProperty rdf:about="http://purl.org/nampi/owl/core#is_authored_on">
        <rdfs:subPropertyOf rdf:resource="http://erlangen-crm.org/211015/P4_has_time-span"/>
        <rdfs:subPropertyOf rdf:resource="http://www.w3.org/2002/07/owl#topObjectProperty"/>
        <rdfs:domain rdf:resource="http://purl.org/nampi/owl/core#act"/>
        <rdfs:range rdf:resource="http://purl.org/nampi/owl/core#date"/>
        <rdfs:comment xml:lang="en">Specifies the date a document interpretation act is authored on.</rdfs:comment>
        <rdfs:label xml:lang="en">is authored on</rdfs:label>
    </owl:ObjectProperty>
    


    <!-- http://purl.org/nampi/owl/core#is_born_in -->

    <owl:ObjectProperty rdf:about="http://purl.org/nampi/owl/core#is_born_in">
        <rdfs:subPropertyOf rdf:resource="http://purl.org/nampi/owl/core#is_main_participant_in"/>
        <owl:inverseOf rdf:resource="http://purl.org/nampi/owl/core#starts_life_of"/>
        <rdfs:comment xml:lang="en">Specifies that the event is about the start of the life of the main participant.</rdfs:comment>
        <rdfs:label xml:lang="en">is born in</rdfs:label>
    </owl:ObjectProperty>
    


    <!-- http://purl.org/nampi/owl/core#is_interpretation_of -->

    <owl:ObjectProperty rdf:about="http://purl.org/nampi/owl/core#is_interpretation_of">
        <rdfs:subPropertyOf rdf:resource="http://erlangen-crm.org/211015/P140i_was_attributed_by"/>
        <rdfs:subPropertyOf rdf:resource="http://www.w3.org/2002/07/owl#topObjectProperty"/>
        <rdfs:comment xml:lang="en">Specifies the event instance that contains the interpretation of the source location in the documentation act</rdfs:comment>
        <rdfs:label xml:lang="en">is interpretation of</rdfs:label>
    </owl:ObjectProperty>
    


    <!-- http://purl.org/nampi/owl/core#is_main_participant_in -->

    <owl:ObjectProperty rdf:about="http://purl.org/nampi/owl/core#is_main_participant_in">
        <rdfs:subPropertyOf rdf:resource="http://purl.org/nampi/owl/core#participates_in"/>
        <rdfs:comment xml:lang="en">Declares a person to be the main participant of a specific event.</rdfs:comment>
        <rdfs:label xml:lang="en">is main participant in</rdfs:label>
    </owl:ObjectProperty>
    


    <!-- http://purl.org/nampi/owl/core#is_other_participant_in -->

    <owl:ObjectProperty rdf:about="http://purl.org/nampi/owl/core#is_other_participant_in">
        <rdfs:subPropertyOf rdf:resource="http://purl.org/nampi/owl/core#participates_in"/>
        <rdfs:comment xml:lang="en">Signifies that an actor is a secondary participant in the real-life event depicted by the event.</rdfs:comment>
        <rdfs:label xml:lang="en">is other participant in</rdfs:label>
    </owl:ObjectProperty>
    


    <!-- http://purl.org/nampi/owl/core#is_parent_in -->

    <owl:ObjectProperty rdf:about="http://purl.org/nampi/owl/core#is_parent_in">
        <rdfs:subPropertyOf rdf:resource="http://purl.org/nampi/owl/core#is_other_participant_in"/>
        <rdfs:comment xml:lang="en">Signifies that the actor functions starts being counted as parent of the main person in the event.</rdfs:comment>
        <rdfs:label xml:lang="en">is parent in</rdfs:label>
    </owl:ObjectProperty>
    


    <!-- http://purl.org/nampi/owl/core#is_part_of -->

    <owl:ObjectProperty rdf:about="http://purl.org/nampi/owl/core#is_part_of">
        <rdfs:subPropertyOf rdf:resource="http://erlangen-crm.org/211015/P107i_is_current_or_former_member_of"/>
        <rdfs:subPropertyOf rdf:resource="http://www.w3.org/2002/07/owl#topObjectProperty"/>
        <rdfs:domain rdf:resource="http://purl.org/nampi/owl/core#actor"/>
        <rdfs:range rdf:resource="http://purl.org/nampi/owl/core#group"/>
        <rdfs:comment xml:lang="en">Specifies a group an actor is part of.</rdfs:comment>
        <rdfs:label xml:lang="en">is part of</rdfs:label>
    </owl:ObjectProperty>
    


    <!-- http://purl.org/nampi/owl/core#is_place_of -->

    <owl:ObjectProperty rdf:about="http://purl.org/nampi/owl/core#is_place_of">
        <rdfs:subPropertyOf rdf:resource="http://erlangen-crm.org/211015/P129i_is_subject_of"/>
        <rdfs:subPropertyOf rdf:resource="http://www.w3.org/2002/07/owl#topObjectProperty"/>
        <owl:inverseOf rdf:resource="http://purl.org/nampi/owl/core#takes_place_at"/>
        <rdfs:comment xml:lang="en">Signifies the place a real-life event depicted in an event took place at.</rdfs:comment>
        <rdfs:label xml:lang="en">is place of</rdfs:label>
    </owl:ObjectProperty>
    


    <!-- http://purl.org/nampi/owl/core#is_related_to_changed_aspect_in -->

    <owl:ObjectProperty rdf:about="http://purl.org/nampi/owl/core#is_related_to_changed_aspect_in">
        <rdfs:subPropertyOf rdf:resource="http://purl.org/nampi/owl/core#is_other_participant_in"/>
        <rdfs:comment xml:lang="en">Signifies that aspects related to the event are also related to the secondary actor. In case of a group, this can mean for instance that a status was valid inside the group or that an occupation had the actor as employer.</rdfs:comment>
        <rdfs:label xml:lang="en">is related to changed aspect in</rdfs:label>
    </owl:ObjectProperty>
    


    <!-- http://purl.org/nampi/owl/core#is_source_location_for -->

    <owl:ObjectProperty rdf:about="http://purl.org/nampi/owl/core#is_source_location_for">
        <rdfs:subPropertyOf rdf:resource="http://erlangen-crm.org/211015/P16i_was_used_for"/>
        <rdfs:subPropertyOf rdf:resource="http://www.w3.org/2002/07/owl#topObjectProperty"/>
        <rdfs:comment xml:lang="en">Speifies the source location a document interpretation act is based on.</rdfs:comment>
        <rdfs:label xml:lang="en">is source location for</rdfs:label>
    </owl:ObjectProperty>
    


    <!-- http://purl.org/nampi/owl/core#participates_in -->

    <owl:ObjectProperty rdf:about="http://purl.org/nampi/owl/core#participates_in">
        <rdfs:subPropertyOf rdf:resource="http://erlangen-crm.org/211015/P129i_is_subject_of"/>
        <rdfs:subPropertyOf rdf:resource="http://www.w3.org/2002/07/owl#topObjectProperty"/>
        <rdfs:comment xml:lang="en">Connects an event to an actor. It means that the actor is in one way or another involved in the real-life event the event depicts.</rdfs:comment>
        <rdfs:label xml:lang="en">participates in</rdfs:label>
    </owl:ObjectProperty>
    


    <!-- http://purl.org/nampi/owl/core#removes_aspect -->

    <owl:ObjectProperty rdf:about="http://purl.org/nampi/owl/core#removes_aspect">
        <rdfs:subPropertyOf rdf:resource="http://purl.org/nampi/owl/core#uses_aspect"/>
        <rdfs:comment xml:lang="en">A pre-existing relationship between the main participant of the event and the aspect is severed. This can mean, for instance, that a status is lost or an occupation is stopped.</rdfs:comment>
        <rdfs:label xml:lang="en">removes aspect</rdfs:label>
    </owl:ObjectProperty>
    


    <!-- http://purl.org/nampi/owl/core#same_as -->

    <owl:ObjectProperty rdf:about="http://purl.org/nampi/owl/core#same_as">
        <rdfs:subPropertyOf rdf:resource="http://www.w3.org/2002/07/owl#topObjectProperty"/>
        <rdfs:comment xml:lang="en">Relates to an entity in an external database that is about the same thing.</rdfs:comment>
        <rdfs:label xml:lang="en">same as</rdfs:label>
    </owl:ObjectProperty>
    


    <!-- http://purl.org/nampi/owl/core#starts_life_of -->

    <owl:ObjectProperty rdf:about="http://purl.org/nampi/owl/core#starts_life_of">
        <rdfs:subPropertyOf rdf:resource="http://purl.org/nampi/owl/core#has_main_participant"/>
        <rdfs:range rdf:resource="http://purl.org/nampi/owl/core#person"/>
        <rdfs:comment xml:lang="en">Specifies that the event is about the start of the life of the main participant.</rdfs:comment>
        <rdfs:label xml:lang="en">starts life of</rdfs:label>
    </owl:ObjectProperty>
    


    <!-- http://purl.org/nampi/owl/core#takes_place_at -->

    <owl:ObjectProperty rdf:about="http://purl.org/nampi/owl/core#takes_place_at">
        <rdfs:subPropertyOf rdf:resource="http://erlangen-crm.org/211015/P129_is_about"/>
        <rdfs:subPropertyOf rdf:resource="http://www.w3.org/2002/07/owl#topObjectProperty"/>
        <rdfs:domain rdf:resource="http://purl.org/nampi/owl/core#event"/>
        <rdfs:range rdf:resource="http://purl.org/nampi/owl/core#place"/>
        <rdfs:comment xml:lang="en">Signifies the place a real-life event depicted in an event took place at.</rdfs:comment>
        <rdfs:label xml:lang="en">takes place at</rdfs:label>
    </owl:ObjectProperty>
    


    <!-- http://purl.org/nampi/owl/core#takes_place_not_earlier_than -->

    <owl:ObjectProperty rdf:about="http://purl.org/nampi/owl/core#takes_place_not_earlier_than">
        <rdfs:subPropertyOf rdf:resource="http://purl.org/nampi/owl/core#has_date"/>
        <rdfs:comment xml:lang="en">Specifies the lower boundary of an unclear event date. Using this means that the specified date is the earliest possible date the real-life event represented in the event could have happened.</rdfs:comment>
        <rdfs:label xml:lang="en">takes place not earlier than</rdfs:label>
    </owl:ObjectProperty>
    


    <!-- http://purl.org/nampi/owl/core#takes_place_not_later_than -->

    <owl:ObjectProperty rdf:about="http://purl.org/nampi/owl/core#takes_place_not_later_than">
        <rdfs:subPropertyOf rdf:resource="http://purl.org/nampi/owl/core#has_date"/>
        <rdfs:comment xml:lang="en">Specifies the upper boundary of an unclear event date. Using this means that the specified date is the latest possible date the real-life event represented in the event could have happened.</rdfs:comment>
        <rdfs:label xml:lang="en">takes place not later than</rdfs:label>
    </owl:ObjectProperty>
    


    <!-- http://purl.org/nampi/owl/core#takes_place_on -->

    <owl:ObjectProperty rdf:about="http://purl.org/nampi/owl/core#takes_place_on">
        <rdfs:subPropertyOf rdf:resource="http://purl.org/nampi/owl/core#has_date"/>
        <rdfs:comment xml:lang="en">Specifies that the real-life event the event depicts has happened exactly on a specific date.</rdfs:comment>
        <rdfs:label xml:lang="en">takes place on</rdfs:label>
    </owl:ObjectProperty>
    


    <!-- http://purl.org/nampi/owl/core#uses_aspect -->

    <owl:ObjectProperty rdf:about="http://purl.org/nampi/owl/core#uses_aspect">
        <rdfs:subPropertyOf rdf:resource="http://erlangen-crm.org/211015/P67_refers_to"/>
        <rdfs:subPropertyOf rdf:resource="http://www.w3.org/2002/07/owl#topObjectProperty"/>
        <rdfs:domain rdf:resource="http://purl.org/nampi/owl/core#event"/>
        <rdfs:range rdf:resource="http://purl.org/nampi/owl/core#aspect"/>
        <rdfs:comment xml:lang="en">Connects an aspect to an event it is relevant to / was used in. Being connected to an event means this aspect is related to the main participant of the event and in a lesser degree to the other participants.</rdfs:comment>
        <rdfs:label xml:lang="en">uses aspect</rdfs:label>
    </owl:ObjectProperty>
    


    <!-- 
    ///////////////////////////////////////////////////////////////////////////////////////
    //
    // Data properties
    //
    ///////////////////////////////////////////////////////////////////////////////////////
     -->

    


    <!-- http://purl.org/nampi/owl/core#has_date_time -->

    <owl:DatatypeProperty rdf:about="http://purl.org/nampi/owl/core#has_date_time">
        <rdfs:subPropertyOf rdf:resource="http://purl.org/nampi/owl/core#has_value"/>
        <rdfs:range rdf:resource="http://www.w3.org/2001/XMLSchema#dateTime"/>
        <rdfs:label xml:lang="en">has dateTime</rdfs:label>
    </owl:DatatypeProperty>
    


    <!-- http://purl.org/nampi/owl/core#has_double -->

    <owl:DatatypeProperty rdf:about="http://purl.org/nampi/owl/core#has_double">
        <rdfs:subPropertyOf rdf:resource="http://purl.org/nampi/owl/core#has_value"/>
        <rdfs:range rdf:resource="http://www.w3.org/2001/XMLSchema#double"/>
        <rdfs:label xml:lang="en">has double</rdfs:label>
    </owl:DatatypeProperty>
    


    <!-- http://purl.org/nampi/owl/core#has_latitude -->

    <owl:DatatypeProperty rdf:about="http://purl.org/nampi/owl/core#has_latitude">
        <rdfs:subPropertyOf rdf:resource="http://purl.org/nampi/owl/core#has_double"/>
        <rdfs:domain rdf:resource="http://purl.org/nampi/owl/core#place"/>
        <rdfs:label xml:lang="en">has longitude</rdfs:label>
    </owl:DatatypeProperty>
    


    <!-- http://purl.org/nampi/owl/core#has_longitude -->

    <owl:DatatypeProperty rdf:about="http://purl.org/nampi/owl/core#has_longitude">
        <rdfs:subPropertyOf rdf:resource="http://purl.org/nampi/owl/core#has_double"/>
        <rdfs:domain rdf:resource="http://purl.org/nampi/owl/core#place"/>
        <rdfs:label xml:lang="en">has latitude</rdfs:label>
    </owl:DatatypeProperty>
    


    <!-- http://purl.org/nampi/owl/core#has_text -->

    <owl:DatatypeProperty rdf:about="http://purl.org/nampi/owl/core#has_text">
        <rdfs:subPropertyOf rdf:resource="http://purl.org/nampi/owl/core#has_value"/>
        <rdfs:label xml:lang="en">has text</rdfs:label>
    </owl:DatatypeProperty>
    


    <!-- http://purl.org/nampi/owl/core#has_value -->

    <owl:DatatypeProperty rdf:about="http://purl.org/nampi/owl/core#has_value">
        <rdfs:subPropertyOf rdf:resource="http://www.w3.org/2002/07/owl#topDataProperty"/>
        <rdfs:label xml:lang="en">has value</rdfs:label>
    </owl:DatatypeProperty>
    


    <!-- 
    ///////////////////////////////////////////////////////////////////////////////////////
    //
    // Classes
    //
    ///////////////////////////////////////////////////////////////////////////////////////
     -->

    


    <!-- http://erlangen-crm.org/211015/E13_Attribute_Assignment -->

    <owl:Class rdf:about="http://erlangen-crm.org/211015/E13_Attribute_Assignment"/>
    


    <!-- http://erlangen-crm.org/211015/E21_Person -->

    <owl:Class rdf:about="http://erlangen-crm.org/211015/E21_Person">
        <owl:equivalentClass rdf:resource="http://purl.org/nampi/owl/core#person"/>
    </owl:Class>
    


    <!-- http://erlangen-crm.org/211015/E39_Actor -->

    <owl:Class rdf:about="http://erlangen-crm.org/211015/E39_Actor">
        <owl:equivalentClass rdf:resource="http://purl.org/nampi/owl/core#actor"/>
    </owl:Class>
    


    <!-- http://erlangen-crm.org/211015/E52_Time-Span -->

    <owl:Class rdf:about="http://erlangen-crm.org/211015/E52_Time-Span"/>
    


    <!-- http://erlangen-crm.org/211015/E53_Place -->

    <owl:Class rdf:about="http://erlangen-crm.org/211015/E53_Place">
        <owl:equivalentClass rdf:resource="http://purl.org/nampi/owl/core#place"/>
    </owl:Class>
    


    <!-- http://erlangen-crm.org/211015/E74_Group -->

    <owl:Class rdf:about="http://erlangen-crm.org/211015/E74_Group">
        <owl:equivalentClass rdf:resource="http://purl.org/nampi/owl/core#group"/>
    </owl:Class>
    


    <!-- http://purl.org/nampi/owl/core#act -->

    <owl:Class rdf:about="http://purl.org/nampi/owl/core#act">
        <rdfs:subClassOf rdf:resource="http://erlangen-crm.org/211015/E13_Attribute_Assignment"/>
        <rdfs:comment xml:lang="en">A document interpretation act as described in Michele Pasin and John Bradley, Factoid-based Prosopography and Computer Ontologies:
Towards an Integrated Approach, in: Digital Scholarship in the Humanities 30 (2015) 86-97.</rdfs:comment>
        <rdfs:label xml:lang="en">Act</rdfs:label>
    </owl:Class>
    


    <!-- http://purl.org/nampi/owl/core#actor -->

    <owl:Class rdf:about="http://purl.org/nampi/owl/core#actor">
        <rdfs:comment xml:lang="en">A person or group of persons or any other entity that is able to affect the world around them with their actions.</rdfs:comment>
        <rdfs:label xml:lang="en">Actor</rdfs:label>
    </owl:Class>
    


    <!-- http://purl.org/nampi/owl/core#appellation -->

    <owl:Class rdf:about="http://purl.org/nampi/owl/core#appellation">
        <rdfs:subClassOf rdf:resource="http://purl.org/nampi/owl/core#aspect"/>
        <rdfs:comment xml:lang="en">Any kind of appellation like names, titles or identifiers.</rdfs:comment>
        <rdfs:label xml:lang="en">Appellation</rdfs:label>
    </owl:Class>
    


    <!-- http://purl.org/nampi/owl/core#aspect -->

    <owl:Class rdf:about="http://purl.org/nampi/owl/core#aspect">
        <rdfs:subClassOf rdf:resource="http://erlangen-crm.org/211015/E70_Thing"/>
        <rdfs:comment xml:lang="en">Anything except actors, places and dates that an event is about. An aspect can be a name gained in an event, a new status, a started occupation, a new posession and all other things that the event impacts. All aspect relevant to an event are directly related to the main participant of an event.</rdfs:comment>
        <rdfs:label xml:lang="en">Aspect</rdfs:label>
    </owl:Class>
    


    <!-- http://purl.org/nampi/owl/core#author -->

    <owl:Class rdf:about="http://purl.org/nampi/owl/core#author">
        <rdfs:subClassOf rdf:resource="http://purl.org/nampi/owl/core#actor"/>
        <rdfs:comment xml:lang="en">An actor that can interpret source locations and create core:events based on their interpretations.</rdfs:comment>
        <rdfs:label xml:lang="en">Author</rdfs:label>
    </owl:Class>
    


    <!-- http://purl.org/nampi/owl/core#date -->

    <owl:Class rdf:about="http://purl.org/nampi/owl/core#date">
        <rdfs:subClassOf rdf:resource="http://erlangen-crm.org/211015/E52_Time-Span"/>
        <rdfs:comment xml:lang="en">A calendar date identifying a specific day.</rdfs:comment>
        <rdfs:label xml:lang="en">Date</rdfs:label>
    </owl:Class>
    


    <!-- http://purl.org/nampi/owl/core#event -->

    <owl:Class rdf:about="http://purl.org/nampi/owl/core#event">
        <rdfs:subClassOf rdf:resource="http://erlangen-crm.org/211015/E89_Propositional_Object"/>
        <rdfs:comment xml:lang="en">A description of the proceedings of an event with a particular focus. This propositional object is part of a single document interpretation act. Real life events can be described by more than one core:event with different main participants, aspects related to different groups and any other view point a particular author might have on the real-life event as described in a particular source.</rdfs:comment>
        <rdfs:label xml:lang="en">Event</rdfs:label>
    </owl:Class>
    


    <!-- http://purl.org/nampi/owl/core#group -->

    <owl:Class rdf:about="http://purl.org/nampi/owl/core#group">
        <rdfs:subClassOf rdf:resource="http://purl.org/nampi/owl/core#actor"/>
        <rdfs:comment xml:lang="en">A group of people. This can be a club, a corporation, a monastic order, a monastic community, a football team, a family or clan or any other group without regards for the specific kind of organization the group might represent in society.</rdfs:comment>
        <rdfs:label xml:lang="en">Group</rdfs:label>
    </owl:Class>
    


    <!-- http://purl.org/nampi/owl/core#identifier -->

    <owl:Class rdf:about="http://purl.org/nampi/owl/core#identifier">
        <rdfs:subClassOf rdf:resource="http://purl.org/nampi/owl/core#appellation"/>
        <rdfs:comment xml:lang="en">An identifier that refers to its object more formally than a name.</rdfs:comment>
        <rdfs:label xml:lang="en">Identifier</rdfs:label>
    </owl:Class>
    


    <!-- http://purl.org/nampi/owl/core#name -->

    <owl:Class rdf:about="http://purl.org/nampi/owl/core#name">
        <rdfs:subClassOf rdf:resource="http://purl.org/nampi/owl/core#appellation"/>
        <rdfs:comment xml:lang="en">A name.</rdfs:comment>
        <rdfs:label xml:lang="en">Name</rdfs:label>
    </owl:Class>
    


    <!-- http://purl.org/nampi/owl/core#occupation -->

    <owl:Class rdf:about="http://purl.org/nampi/owl/core#occupation">
        <rdfs:subClassOf rdf:resource="http://purl.org/nampi/owl/core#aspect"/>
        <rdfs:comment xml:lang="en">An occupation like a hobby, trade or craft.</rdfs:comment>
        <rdfs:label xml:lang="en">Occupation</rdfs:label>
    </owl:Class>
    


    <!-- http://purl.org/nampi/owl/core#online_source -->

    <owl:Class rdf:about="http://purl.org/nampi/owl/core#online_source">
        <rdfs:subClassOf rdf:resource="http://purl.org/nampi/owl/core#source"/>
        <rdfs:comment xml:lang="en">Any online source. This can be a website, online data base or other mainly online document.</rdfs:comment>
        <rdfs:label xml:lang="en">Online source</rdfs:label>
    </owl:Class>
    


    <!-- http://purl.org/nampi/owl/core#person -->

    <owl:Class rdf:about="http://purl.org/nampi/owl/core#person">
        <rdfs:subClassOf rdf:resource="http://purl.org/nampi/owl/core#actor"/>
        <rdfs:comment xml:lang="en">A person that is currently alive or has been alive at some point in the past. Imaginary or legendary figures can be included if so desired.</rdfs:comment>
        <rdfs:label xml:lang="en">Person</rdfs:label>
    </owl:Class>
    


    <!-- http://purl.org/nampi/owl/core#place -->

    <owl:Class rdf:about="http://purl.org/nampi/owl/core#place">
        <rdfs:comment xml:lang="en">A geographical place.</rdfs:comment>
        <rdfs:label xml:lang="en">Place</rdfs:label>
    </owl:Class>
    


    <!-- http://purl.org/nampi/owl/core#source -->

    <owl:Class rdf:about="http://purl.org/nampi/owl/core#source">
        <rdfs:subClassOf rdf:resource="http://erlangen-crm.org/211015/E31_Document"/>
        <rdfs:comment xml:lang="en">Any document, analogue or digital, that functions as a source for interpretations in a document interpretation act. This means the whole object not individual sections like pages or single websites.</rdfs:comment>
        <rdfs:label xml:lang="en">Source</rdfs:label>
    </owl:Class>
    


    <!-- http://purl.org/nampi/owl/core#source_location -->

    <owl:Class rdf:about="http://purl.org/nampi/owl/core#source_location">
        <rdfs:subClassOf rdf:resource="http://erlangen-crm.org/211015/E73_Information_Object"/>
        <rdfs:comment xml:lang="en">A specific location inside a source.</rdfs:comment>
        <rdfs:label xml:lang="en">Source location</rdfs:label>
    </owl:Class>
    


    <!-- http://purl.org/nampi/owl/core#status -->

    <owl:Class rdf:about="http://purl.org/nampi/owl/core#status">
        <rdfs:subClassOf rdf:resource="http://purl.org/nampi/owl/core#aspect"/>
        <rdfs:comment xml:lang="en">A social status relevant to the members of a particular group.</rdfs:comment>
        <rdfs:label xml:lang="en">Status</rdfs:label>
    </owl:Class>
    


    <!-- http://purl.org/nampi/owl/core#title -->

    <owl:Class rdf:about="http://purl.org/nampi/owl/core#title">
        <rdfs:subClassOf rdf:resource="http://purl.org/nampi/owl/core#appellation"/>
        <rdfs:comment xml:lang="en">A formal title that refers to an individual.</rdfs:comment>
        <rdfs:label xml:lang="en">Title</rdfs:label>
    </owl:Class>
</rdf:RDF>



<!-- Generated by the OWL API (version 4.5.9.2019-02-01T07:24:44Z) https://github.com/owlcs/owlapi -->

